Update Coq prover snapshot

prover_snapshots/coq/lib/sail/Prompt.v
@@ -1,3 +1,70 @@
+(*==========================================================================*)
+(*     Sail                                                                 *)
+(*                                                                          *)
+(*  Sail and the Sail architecture models here, comprising all files and    *)
+(*  directories except the ASL-derived Sail code in the aarch64 directory,  *)
+(*  are subject to the BSD two-clause licence below.                        *)
+(*                                                                          *)
+(*  The ASL derived parts of the ARMv8.3 specification in                   *)
+(*  aarch64/no_vector and aarch64/full are copyright ARM Ltd.               *)
+(*                                                                          *)
+(*  Copyright (c) 2013-2021                                                 *)
+(*    Kathyrn Gray                                                          *)
+(*    Shaked Flur                                                           *)
+(*    Stephen Kell                                                          *)
+(*    Gabriel Kerneis                                                       *)
+(*    Robert Norton-Wright                                                  *)
+(*    Christopher Pulte                                                     *)
+(*    Peter Sewell                                                          *)
+(*    Alasdair Armstrong                                                    *)
+(*    Brian Campbell                                                        *)
+(*    Thomas Bauereiss                                                      *)
+(*    Anthony Fox                                                           *)
+(*    Jon French                                                            *)
+(*    Dominic Mulligan                                                      *)
+(*    Stephen Kell                                                          *)
+(*    Mark Wassell                                                          *)
+(*    Alastair Reid (Arm Ltd)                                               *)
+(*                                                                          *)
+(*  All rights reserved.                                                    *)
+(*                                                                          *)
+(*  This work was partially supported by EPSRC grant EP/K008528/1 <a        *)
+(*  href="http://www.cl.cam.ac.uk/users/pes20/rems">REMS: Rigorous          *)
+(*  Engineering for Mainstream Systems</a>, an ARM iCASE award, EPSRC IAA   *)
+(*  KTF funding, and donations from Arm.  This project has received         *)
+(*  funding from the European Research Council (ERC) under the European     *)
+(*  Union’s Horizon 2020 research and innovation programme (grant           *)
+(*  agreement No 789108, ELVER).                                            *)
+(*                                                                          *)
+(*  This software was developed by SRI International and the University of  *)
+(*  Cambridge Computer Laboratory (Department of Computer Science and       *)
+(*  Technology) under DARPA/AFRL contracts FA8650-18-C-7809 ("CIFV")        *)
+(*  and FA8750-10-C-0237 ("CTSRD").                                         *)
+(*                                                                          *)
+(*  Redistribution and use in source and binary forms, with or without      *)
+(*  modification, are permitted provided that the following conditions      *)
+(*  are met:                                                                *)
+(*  1. Redistributions of source code must retain the above copyright       *)
+(*     notice, this list of conditions and the following disclaimer.        *)
+(*  2. Redistributions in binary form must reproduce the above copyright    *)
+(*     notice, this list of conditions and the following disclaimer in      *)
+(*     the documentation and/or other materials provided with the           *)
+(*     distribution.                                                        *)
+(*                                                                          *)
+(*  THIS SOFTWARE IS PROVIDED BY THE AUTHOR AND CONTRIBUTORS ``AS IS''      *)
+(*  AND ANY EXPRESS OR IMPLIED WARRANTIES, INCLUDING, BUT NOT LIMITED       *)
+(*  TO, THE IMPLIED WARRANTIES OF MERCHANTABILITY AND FITNESS FOR A         *)
+(*  PARTICULAR PURPOSE ARE DISCLAIMED.  IN NO EVENT SHALL THE AUTHOR OR     *)
+(*  CONTRIBUTORS BE LIABLE FOR ANY DIRECT, INDIRECT, INCIDENTAL,            *)
+(*  SPECIAL, EXEMPLARY, OR CONSEQUENTIAL DAMAGES (INCLUDING, BUT NOT        *)
+(*  LIMITED TO, PROCUREMENT OF SUBSTITUTE GOODS OR SERVICES; LOSS OF        *)
+(*  USE, DATA, OR PROFITS; OR BUSINESS INTERRUPTION) HOWEVER CAUSED AND     *)
+(*  ON ANY THEORY OF LIABILITY, WHETHER IN CONTRACT, STRICT LIABILITY,      *)
+(*  OR TORT (INCLUDING NEGLIGENCE OR OTHERWISE) ARISING IN ANY WAY OUT      *)
+(*  OF THE USE OF THIS SOFTWARE, EVEN IF ADVISED OF THE POSSIBILITY OF      *)
+(*  SUCH DAMAGE.                                                            *)
+(*==========================================================================*)
+
 Require Import Sail.Values.
 Require Import Sail.Prompt_monad.
 Require Export ZArith.Zwf.
@@ -31,30 +98,55 @@ match l with
   foreachM xs vars body
 end.
 
-Fixpoint foreach_ZM_up' {rv e Vars} (from to step off : Z) (n : nat) `{ArithFact (0 <? step)} `{ArithFact (0 <=? off)} (vars : Vars) (body : forall (z : Z) `(ArithFact (from <=? z <=? to)), Vars -> monad rv Vars e) {struct n} : monad rv Vars e.
-exact (
+Fixpoint foreachE {a Vars e} (l : list a) (vars : Vars) (body : a -> Vars -> e + Vars) : e + Vars :=
+match l with
+| [] => inr vars
+| (x :: xs) =>
+  body x vars >>$= fun vars =>
+  foreachE xs vars body
+end.
+
+Fixpoint foreach_ZM_up' {rv e Vars} (from to step off : Z) (n : nat) (* 0 <? step *) (* 0 <=? off *) (vars : Vars) (body : forall (z : Z) (* from <=? z <=? to *), Vars -> monad rv Vars e) {struct n} : monad rv Vars e :=
   if sumbool_of_bool (from + off <=? to) then
     match n with
     | O => returnm vars
-    | S n => body (from + off) _ vars >>= fun vars => foreach_ZM_up' rv e Vars from to step (off + step) n _ _ vars body
+    | S n => body (from + off) vars >>= fun vars => foreach_ZM_up' from to step (off + step) n vars body
     end
-  else returnm vars).
-Defined.
+  else returnm vars.
 
-Fixpoint foreach_ZM_down' {rv e Vars} (from to step off : Z) (n : nat) `{ArithFact (0 <? step)} `{ArithFact (off <=? 0)} (vars : Vars) (body : forall (z : Z) `(ArithFact (to <=? z <=? from)), Vars -> monad rv Vars e) {struct n} : monad rv Vars e.
-exact (
+Fixpoint foreach_ZE_up' {e Vars} (from to step off : Z) (n : nat) (* 0 <? step *) (* 0 <=? off *) (vars : Vars) (body : forall (z : Z) (* from <=? z <=? to *), Vars -> e + Vars) {struct n} : e + Vars :=
+  if sumbool_of_bool (from + off <=? to) then
+    match n with
+    | O => inr vars
+    | S n => body (from + off) vars >>$= fun vars => foreach_ZE_up' from to step (off + step) n vars body
+    end
+  else inr vars.
+
+Fixpoint foreach_ZM_down' {rv e Vars} (from to step off : Z) (n : nat) (* 0 <? step *) (* off <=? 0 *) (vars : Vars) (body : forall (z : Z) (* to <=? z <=? from *), Vars -> monad rv Vars e) {struct n} : monad rv Vars e :=
   if sumbool_of_bool (to <=? from + off) then
     match n with
     | O => returnm vars
-    | S n => body (from + off) _ vars >>= fun vars => foreach_ZM_down' _ _ _ from to step (off - step) n _ _ vars body
+    | S n => body (from + off) vars >>= fun vars => foreach_ZM_down' from to step (off - step) n vars body
     end
-  else returnm vars).
-Defined.
+  else returnm vars.
 
-Definition foreach_ZM_up {rv e Vars} from to step vars body `{ArithFact (0 <? step)} :=
+Fixpoint foreach_ZE_down' {e Vars} (from to step off : Z) (n : nat) (* 0 <? step *) (* off <=? 0 *) (vars : Vars) (body : forall (z : Z) (* to <=? z <=? from *), Vars -> e + Vars) {struct n} : e + Vars :=
+  if sumbool_of_bool (to <=? from + off) then
+    match n with
+    | O => inr vars
+    | S n => body (from + off) vars >>$= fun vars => foreach_ZE_down' from to step (off - step) n vars body
+    end
+  else inr vars.
+
+Definition foreach_ZM_up {rv e Vars} from to step vars body (* 0 <? step *) :=
     foreach_ZM_up' (rv := rv) (e := e) (Vars := Vars) from to step 0 (S (Z.abs_nat (from - to))) vars body.
-Definition foreach_ZM_down {rv e Vars} from to step vars body `{ArithFact (0 <? step)} :=
+Definition foreach_ZM_down {rv e Vars} from to step vars body (* 0 <? step *) :=
     foreach_ZM_down' (rv := rv) (e := e) (Vars := Vars) from to step 0 (S (Z.abs_nat (from - to))) vars body.
+
+Definition foreach_ZE_up {e Vars} from to step vars body (* 0 <? step *) :=
+    foreach_ZE_up' (e := e) (Vars := Vars) from to step 0 (S (Z.abs_nat (from - to))) vars body.
+Definition foreach_ZE_down {e Vars} from to step vars body (* 0 <? step *) :=
+    foreach_ZE_down' (e := e) (Vars := Vars) from to step 0 (S (Z.abs_nat (from - to))) vars body.
 
 (*declare {isabelle} termination_argument foreachM = automatic*)
 
@@ -73,7 +165,7 @@ Definition and_bool_left_proof {P Q R:bool -> Prop} :
   ArithFactP (P false) ->
   (forall l r, ArithFactP (P l -> ((l = true -> (Q r)) -> (R (andb l r))))) ->
   ArithFactP (R false).
-intros [p] [h].
+intros [p] h.
 constructor.
 change false with (andb false false).
 apply h; auto.
@@ -85,7 +177,7 @@ Definition and_bool_full_proof {P Q R:bool -> Prop} {r} :
   ArithFactP (Q r) ->
   (forall l r, ArithFactP ((P l) -> ((l = true -> (Q r)) -> (R (andb l r))))) ->
   ArithFactP (R r).
-intros [p] [q] [h].
+intros [p] [q] h.
 constructor.
 change r with (andb true r).
 apply h; auto.
@@ -94,9 +186,9 @@ Qed.
 Definition and_boolMP {rv E} {P Q R:bool->Prop} (x : monad rv {b:bool & ArithFactP (P b)} E) (y : monad rv {b:bool & ArithFactP (Q b)} E)
   `{H:forall l r, ArithFactP ((P l) -> ((l = true -> (Q r)) -> (R (andb l r))))}
   : monad rv {b:bool & ArithFactP (R b)} E :=
-  x >>= fun '(existT _ x p) => (if x return ArithFactP (P x) -> _ then
-    fun p => y >>= fun '(existT _ y q) => returnm (existT _ y (and_bool_full_proof p q H))
-  else fun p => returnm (existT _ false (and_bool_left_proof p H))) p.
+  x >>= fun '(@existT _ _ x p) => (if x return ArithFactP (P x) -> _ then
+    fun p => y >>= fun '(@existT _ _ y q) => returnm (@existT _ _ y (and_bool_full_proof p q H))
+  else fun p => returnm (@existT _ _ false (and_bool_left_proof p H))) p.
 
 (*val or_boolM : forall 'rv 'e. monad 'rv bool 'e -> monad 'rv bool 'e -> monad 'rv bool 'e*)
 Definition or_boolM {rv E} (l : monad rv bool E) (r : monad rv bool E) : monad rv bool E :=
@@ -107,7 +199,7 @@ Definition or_bool_left_proof {P Q R:bool -> Prop} :
   ArithFactP (P true) ->
   (forall l r, ArithFactP ((P l) -> (((l = false) -> (Q r)) -> (R (orb l r))))) ->
   ArithFactP (R true).
-intros [p] [h].
+intros [p] h.
 constructor.
 change true with (orb true false).
 apply h; auto.
@@ -119,7 +211,7 @@ Definition or_bool_full_proof {P Q R:bool -> Prop} {r} :
   ArithFactP (Q r) ->
   (forall l r, ArithFactP ((P l) -> (((l = false) -> (Q r)) -> (R (orb l r))))) ->
   ArithFactP (R r).
-intros [p] [q] [h].
+intros [p] [q] h.
 constructor.
 change r with (orb false r).
 apply h; auto.
@@ -128,12 +220,12 @@ Qed.
 Definition or_boolMP {rv E} {P Q R:bool -> Prop} (l : monad rv {b : bool & ArithFactP (P b)} E) (r : monad rv {b : bool & ArithFactP (Q b)} E)
  `{forall l r, ArithFactP ((P l) -> (((l = false) -> (Q r)) -> (R (orb l r))))}
  : monad rv {b : bool & ArithFactP (R b)} E :=
- l >>= fun '(existT _ l p) =>
-  (if l return ArithFactP (P l) -> _ then fun p => returnm (existT _ true (or_bool_left_proof p H))
-   else fun p => r >>= fun '(existT _ r q) => returnm (existT _ r (or_bool_full_proof p q H))) p.
+ l >>= fun '(@existT _ _ l p) =>
+  (if l return ArithFactP (P l) -> _ then fun p => returnm (@existT _ _ true (or_bool_left_proof p H))
+   else fun p => r >>= fun '(@existT _ _ r q) => returnm (@existT _ _ r (or_bool_full_proof p q H))) p.
 
 Definition build_trivial_ex {rv E} {T:Type} (x:monad rv T E) : monad rv {x : T & ArithFact true} E :=
-  x >>= fun x => returnm (existT _ x (Build_ArithFactP _ eq_refl)).
+  x >>= fun x => returnm (@existT _ _ x (Build_ArithFactP _ eq_refl)).
 
 (*val bool_of_bitU_fail : forall 'rv 'e. bitU -> monad 'rv bool 'e*)
 Definition bool_of_bitU_fail {rv E} (b : bitU) : monad rv bool E :=
@@ -156,11 +248,11 @@ Definition bools_of_bits_nondet {rv E} (bits : list bitU) : monad rv (list bool)
       bool_of_bitU_nondet b >>= fun b => 
       returnm (bools ++ [b])).
 
-Definition of_bits_nondet {rv A E} `{Bitvector A} (bits : list bitU) : monad rv A E :=
+Definition of_bits_nondet {rv n E} (bits : list bitU) `{ArithFact (n >=? 0)} : monad rv (mword n) E :=
   bools_of_bits_nondet bits >>= fun bs =>
   returnm (of_bools bs).
 
-Definition of_bits_fail {rv A E} `{Bitvector A} (bits : list bitU) : monad rv A E :=
+Definition of_bits_fail {rv n E} (bits : list bitU) `{ArithFact (n >=? 0)} : monad rv (mword n) E :=
   maybe_fail "of_bits" (of_bits bits).
 
 (* For termination of recursive functions.  We don't name assertions, so use
@@ -246,43 +338,31 @@ Definition untilMT {RV Vars E} (vars : Vars) (measure : Vars -> Z) (cond : Vars 
     else slice vec (start_vec - size_r1) (start_vec - size_vec) in
   write_reg r1 r1_v >> write_reg r2 r2_v*)
 
-Definition choose_bools {RV E} (descr : string) (n : nat) : monad RV (list bool) E :=
-  genlistM (fun _ => choose_bool descr) n.
+Section Choose.
+Context {rv E : Type}.
 
-Definition choose {RV A E} (descr : string) (xs : list A) : monad RV A E :=
+Definition choose_from_list {A} (descr : string) (xs : list A) : monad rv A E :=
   (* Use sufficiently many nondeterministically chosen bits and convert into an
      index into the list *)
-  choose_bools descr (List.length xs) >>= fun bs =>
-  let idx := ((nat_of_bools bs) mod List.length xs)%nat in
-  match List.nth_error xs idx with
+  choose_range descr 0 (Z.of_nat (List.length xs) - 1) >>= fun idx =>
+  match List.nth_error xs (Z.to_nat idx) with
     | Some x => returnm x
     | None => Fail ("choose " ++ descr)
   end.
 
-Definition internal_pick {rv a e} (xs : list a) : monad rv a e :=
-  choose "internal_pick" xs.
+Definition internal_pick {a} (xs : list a) : monad rv a E :=
+  choose_from_list "internal_pick" xs.
 
-Fixpoint undefined_word_nat {rv e} n : monad rv (Word.word n) e :=
-  match n with
-  | O => returnm Word.WO
-  | S m =>
-    choose_bool "undefined_word_nat" >>= fun b =>
-    undefined_word_nat m >>= fun t =>
-    returnm (Word.WS b t)
-  end.
-
-Definition undefined_bitvector {rv e} n `{ArithFact (n >=? 0)} : monad rv (mword n) e :=
-  undefined_word_nat (Z.to_nat n) >>= fun w =>
-  returnm (word_to_mword w).
+End Choose.
 
 (* If we need to build an existential after a monadic operation, assume that
    we can do it entirely from the type. *)
 
 Definition build_ex_m {rv e} {T:Type} (x:monad rv T e) {P:T -> Prop} `{H:forall x, ArithFactP (P x)} : monad rv {x : T & ArithFactP (P x)} e :=
-  x >>= fun y => returnm (existT _ y (H y)).
+  x >>= fun y => returnm (@existT _ _ y (H y)).
 
 Definition projT1_m {rv e} {T:Type} {P:T -> Prop} (x: monad rv {x : T & P x} e) : monad rv T e :=
   x >>= fun y => returnm (projT1 y).
 
-Definition derive_m {rv e} {T:Type} {P Q:T -> Prop} (x : monad rv {x : T & ArithFactP (P x)} e) `{forall x, ArithFactP (P x) -> ArithFactP (Q x)} : monad rv {x : T & (ArithFactP (Q x))} e :=
-  x >>= fun y => returnm (build_ex (projT1 y)).
+Definition derive_m {rv e} {T:Type} {P Q:T -> Prop} (x : monad rv {x : T & ArithFactP (P x)} e) `{H:forall x, ArithFactP (P x) -> ArithFactP (Q x)} : monad rv {x : T & (ArithFactP (Q x))} e :=
+  x >>= fun y => returnm (@existT _ _ (projT1 y) (H (projT1 y) (projT2 y))).
