prover_snapshots/coq/lib/sail/Prompt_monad.v
@@ -1,30 +1,97 @@
+(*==========================================================================*)
+(*     Sail                                                                 *)
+(*                                                                          *)
+(*  Sail and the Sail architecture models here, comprising all files and    *)
+(*  directories except the ASL-derived Sail code in the aarch64 directory,  *)
+(*  are subject to the BSD two-clause licence below.                        *)
+(*                                                                          *)
+(*  The ASL derived parts of the ARMv8.3 specification in                   *)
+(*  aarch64/no_vector and aarch64/full are copyright ARM Ltd.               *)
+(*                                                                          *)
+(*  Copyright (c) 2013-2021                                                 *)
+(*    Kathyrn Gray                                                          *)
+(*    Shaked Flur                                                           *)
+(*    Stephen Kell                                                          *)
+(*    Gabriel Kerneis                                                       *)
+(*    Robert Norton-Wright                                                  *)
+(*    Christopher Pulte                                                     *)
+(*    Peter Sewell                                                          *)
+(*    Alasdair Armstrong                                                    *)
+(*    Brian Campbell                                                        *)
+(*    Thomas Bauereiss                                                      *)
+(*    Anthony Fox                                                           *)
+(*    Jon French                                                            *)
+(*    Dominic Mulligan                                                      *)
+(*    Stephen Kell                                                          *)
+(*    Mark Wassell                                                          *)
+(*    Alastair Reid (Arm Ltd)                                               *)
+(*                                                                          *)
+(*  All rights reserved.                                                    *)
+(*                                                                          *)
+(*  This work was partially supported by EPSRC grant EP/K008528/1 <a        *)
+(*  href="http://www.cl.cam.ac.uk/users/pes20/rems">REMS: Rigorous          *)
+(*  Engineering for Mainstream Systems</a>, an ARM iCASE award, EPSRC IAA   *)
+(*  KTF funding, and donations from Arm.  This project has received         *)
+(*  funding from the European Research Council (ERC) under the European     *)
+(*  Union’s Horizon 2020 research and innovation programme (grant           *)
+(*  agreement No 789108, ELVER).                                            *)
+(*                                                                          *)
+(*  This software was developed by SRI International and the University of  *)
+(*  Cambridge Computer Laboratory (Department of Computer Science and       *)
+(*  Technology) under DARPA/AFRL contracts FA8650-18-C-7809 ("CIFV")        *)
+(*  and FA8750-10-C-0237 ("CTSRD").                                         *)
+(*                                                                          *)
+(*  Redistribution and use in source and binary forms, with or without      *)
+(*  modification, are permitted provided that the following conditions      *)
+(*  are met:                                                                *)
+(*  1. Redistributions of source code must retain the above copyright       *)
+(*     notice, this list of conditions and the following disclaimer.        *)
+(*  2. Redistributions in binary form must reproduce the above copyright    *)
+(*     notice, this list of conditions and the following disclaimer in      *)
+(*     the documentation and/or other materials provided with the           *)
+(*     distribution.                                                        *)
+(*                                                                          *)
+(*  THIS SOFTWARE IS PROVIDED BY THE AUTHOR AND CONTRIBUTORS ``AS IS''      *)
+(*  AND ANY EXPRESS OR IMPLIED WARRANTIES, INCLUDING, BUT NOT LIMITED       *)
+(*  TO, THE IMPLIED WARRANTIES OF MERCHANTABILITY AND FITNESS FOR A         *)
+(*  PARTICULAR PURPOSE ARE DISCLAIMED.  IN NO EVENT SHALL THE AUTHOR OR     *)
+(*  CONTRIBUTORS BE LIABLE FOR ANY DIRECT, INDIRECT, INCIDENTAL,            *)
+(*  SPECIAL, EXEMPLARY, OR CONSEQUENTIAL DAMAGES (INCLUDING, BUT NOT        *)
+(*  LIMITED TO, PROCUREMENT OF SUBSTITUTE GOODS OR SERVICES; LOSS OF        *)
+(*  USE, DATA, OR PROFITS; OR BUSINESS INTERRUPTION) HOWEVER CAUSED AND     *)
+(*  ON ANY THEORY OF LIABILITY, WHETHER IN CONTRACT, STRICT LIABILITY,      *)
+(*  OR TORT (INCLUDING NEGLIGENCE OR OTHERWISE) ARISING IN ANY WAY OUT      *)
+(*  OF THE USE OF THIS SOFTWARE, EVEN IF ADVISED OF THE POSSIBILITY OF      *)
+(*  SUCH DAMAGE.                                                            *)
+(*==========================================================================*)
+
 Require Import String.
 (*Require Import Sail_impl_base*)
 Require Import Sail.Instr_kinds.
 Require Import Sail.Values.
-Require bbv.Word.
 Import ListNotations.
 Local Open Scope Z.
 
 Definition register_name := string.
-Definition address := list bitU.
+Definition address := N.
 
 Inductive monad regval a e :=
   | Done : a -> monad regval a e
   (* Read a number of bytes from memory, returned in little endian order,
      with or without a tag.  The first nat specifies the address, the second
      the number of bytes. *)
-  | Read_mem : read_kind -> nat -> nat -> (list memory_byte -> monad regval a e) -> monad regval a e
-  | Read_memt : read_kind -> nat -> nat -> ((list memory_byte * bitU) -> monad regval a e) -> monad regval a e
+  | Read_mem : read_kind -> N -> nat -> (list memory_byte -> monad regval a e) -> monad regval a e
+  | Read_memt : read_kind -> N -> nat -> ((list memory_byte * bitU) -> monad regval a e) -> monad regval a e
   (* Tell the system a write is imminent, at the given address and with the
      given size. *)
-  | Write_ea : write_kind -> nat -> nat -> monad regval a e -> monad regval a e
+  | Write_ea : write_kind -> N -> nat -> monad regval a e -> monad regval a e
   (* Request the result : store-exclusive *)
   | Excl_res : (bool -> monad regval a e) -> monad regval a e
   (* Request to write a memory value of the given size at the given address,
      with or without a tag. *)
-  | Write_mem : write_kind -> nat -> nat -> list memory_byte -> (bool -> monad regval a e) -> monad regval a e
-  | Write_memt : write_kind -> nat -> nat -> list memory_byte -> bitU -> (bool -> monad regval a e) -> monad regval a e
+  | Write_mem : write_kind -> N -> nat -> list memory_byte -> (bool -> monad regval a e) -> monad regval a e
+  | Write_memt : write_kind -> N -> nat -> list memory_byte -> bitU -> (bool -> monad regval a e) -> monad regval a e
+  | Write_tag : write_kind -> N -> bitU -> (bool -> monad regval a e) -> monad regval a e
   (* Tell the system to dynamically recalculate dependency footprint *)
   | Footprint : monad regval a e -> monad regval a e
   (* Request a memory barrier *)
@@ -36,7 +103,7 @@ Inductive monad regval a e :=
   (* Request to choose a Boolean, e.g. to resolve an undefined bit. The string
      argument may be used to provide information to the system about what the
      Boolean is going to be used for. *)
-  | Choose : string -> (bool -> monad regval a e) -> monad regval a e
+  | Choose : string -> forall ty, (choose_type ty -> monad regval a e) -> monad regval a e
   (* Print debugging or tracing information *)
   | Print : string -> monad regval a e -> monad regval a e
   (*Result of a failed assert with possible error message to report*)
@@ -51,6 +118,7 @@ Arguments Write_ea [_ _ _].
 Arguments Excl_res [_ _ _].
 Arguments Write_mem [_ _ _].
 Arguments Write_memt [_ _ _].
+Arguments Write_tag [_ _ _].
 Arguments Footprint [_ _ _].
 Arguments Barrier [_ _ _].
 Arguments Read_reg [_ _ _].
@@ -60,18 +128,29 @@ Arguments Print [_ _ _].
 Arguments Fail [_ _ _].
 Arguments Exception [_ _ _].
 
+(* The injectivity tactic can be confused by dependent types when some of the types
+   involved don't quite match syntactically.  Sometimes it's easier to apply a lemma
+   to a hypothesis instead. *)
+Lemma Choose_injective {rv A E} s ty (x y : choose_type ty -> monad rv A E) :
+  Choose s ty x = Choose s ty y ->
+  x = y.
+intros [=].
+assumption.
+Qed.
+
 Inductive event {regval} :=
-  | E_read_mem : read_kind -> nat -> nat -> list memory_byte -> event
-  | E_read_memt : read_kind -> nat -> nat -> (list memory_byte * bitU) -> event
-  | E_write_mem : write_kind -> nat -> nat -> list memory_byte -> bool -> event
-  | E_write_memt : write_kind -> nat -> nat -> list memory_byte -> bitU -> bool -> event
-  | E_write_ea : write_kind -> nat -> nat -> event
+  | E_read_mem : read_kind -> N -> nat -> list memory_byte -> event
+  | E_read_memt : read_kind -> N -> nat -> (list memory_byte * bitU) -> event
+  | E_write_mem : write_kind -> N -> nat -> list memory_byte -> bool -> event
+  | E_write_memt : write_kind -> N -> nat -> list memory_byte -> bitU -> bool -> event
+  | E_write_tag : write_kind -> N -> nat -> bitU -> bool -> event
+  | E_write_ea : write_kind -> N -> nat -> event
   | E_excl_res : bool -> event
   | E_barrier : barrier_kind -> event
   | E_footprint : event
   | E_read_reg : register_name -> regval -> event
   | E_write_reg : register_name -> regval -> event
-  | E_choose : string -> bool -> event
+  | E_choose : string -> forall ty, choose_type ty -> event
   | E_print : string -> event.
 Arguments event : clear implicits.
 
@@ -87,9 +166,10 @@ Fixpoint bind {rv A B E} (m : monad rv A E) (f : A -> monad rv B E) := match m w
   | Read_memt rk a sz k =>      Read_memt rk a sz      (fun v => bind (k v) f)
   | Write_mem wk a sz v k =>    Write_mem wk a sz v    (fun v => bind (k v) f)
   | Write_memt wk a sz v t k => Write_memt wk a sz v t (fun v => bind (k v) f)
+  | Write_tag wk a t k =>       Write_tag wk a t       (fun v => bind (k v) f)
   | Read_reg descr k =>         Read_reg descr         (fun v => bind (k v) f)
   | Excl_res k =>               Excl_res               (fun v => bind (k v) f)
-  | Choose descr k =>           Choose descr           (fun v => bind (k v) f)
+  | Choose descr ty k =>        Choose descr ty        (fun v => bind (k v) f)
   | Write_ea wk a sz k =>       Write_ea wk a sz       (bind k f)
   | Footprint k =>              Footprint              (bind k f)
   | Barrier bk k =>             Barrier bk             (bind k f)
@@ -108,13 +188,30 @@ Notation "m >> n" := (bind0 m n) (at level 50, left associativity).
 (*val exit : forall rv a e. unit -> monad rv a e*)
 Definition exit {rv A E} (_ : unit) : monad rv A E := Fail "exit".
 
+(*val maybe_fail : forall 'rv 'a 'e. string -> maybe 'a -> monad 'rv 'a 'e*)
+Definition maybe_fail {rv A E} msg (x : option A) : monad rv A E :=
+match x with
+  | Some a => returnm a
+  | None => Fail msg
+end.
+
+Section Choose.
+Context {rv E : Type}.
+
 (*val choose_bool : forall 'rv 'e. string -> monad 'rv bool 'e*)
-Definition choose_bool {rv E} descr : monad rv bool E := Choose descr returnm.
+Definition choose_bool descr : monad rv bool E := Choose descr ChooseBool returnm.
+Definition choose_bit descr : monad rv bitU E := Choose descr ChooseBit returnm.
+Definition choose_int descr : monad rv Z E := Choose descr ChooseInt returnm.
+Definition choose_nat descr : monad rv Z E := Choose descr ChooseNat returnm.
+Definition choose_real descr : monad rv _ E := Choose descr ChooseReal returnm.
+Definition choose_string descr : monad rv string E := Choose descr ChooseString returnm.
+Definition choose_range descr lo hi : monad rv Z E :=
+  if lo <=? hi
+  then Choose descr (ChooseRange lo hi) (fun v => if sumbool_of_bool ((lo <=? v) && (v <=? hi)) then returnm v else Fail "choose_range: Bad value")
+  else Fail "choose_range: Bad range".
+Definition choose_bitvector descr n : monad rv (mword n) E := Choose descr (ChooseBitvector n) returnm.
 
-(*val undefined_bool : forall 'rv 'e. unit -> monad 'rv bool 'e*)
-Definition undefined_bool {rv e} (_:unit) : monad rv bool e := choose_bool "undefined_bool".
-
-Definition undefined_unit {rv e} (_:unit) : monad rv unit e := returnm tt.
+End Choose.
 
 (*val assert_exp : forall rv e. bool -> string -> monad rv unit e*)
 Definition assert_exp {rv E} (exp :bool) msg : monad rv unit E :=
@@ -136,9 +233,10 @@ Fixpoint try_catch {rv A E1 E2} (m : monad rv A E1) (h : E1 -> monad rv A E2) :=
   | Read_memt rk a sz k =>      Read_memt rk a sz      (fun v => try_catch (k v) h)
   | Write_mem wk a sz v k =>    Write_mem wk a sz v    (fun v => try_catch (k v) h)
   | Write_memt wk a sz v t k => Write_memt wk a sz v t (fun v => try_catch (k v) h)
+  | Write_tag wk a t k =>       Write_tag wk a t       (fun v => try_catch (k v) h)
   | Read_reg descr k =>         Read_reg descr         (fun v => try_catch (k v) h)
   | Excl_res k =>               Excl_res               (fun v => try_catch (k v) h)
-  | Choose descr k =>           Choose descr           (fun v => try_catch (k v) h)
+  | Choose descr ty k =>        Choose descr ty        (fun v => try_catch (k v) h)
   | Write_ea wk a sz k =>       Write_ea wk a sz       (try_catch k h)
   | Footprint k =>              Footprint              (try_catch k h)
   | Barrier bk k =>             Barrier bk             (try_catch k h)
@@ -164,6 +262,23 @@ Definition catch_early_return {rv A E} (m : monadR rv A A E) :=
       | inr e => throw e
      end).
 
+(* Pure functions with early return using a sum: *)
+
+Definition pure_early_return_bind {A B E} (v : E + A) (f : A -> E + B) : E + B :=
+  match v with
+  | inl e => inl e
+  | inr a => f a
+  end.
+
+Notation "m >>$= f" := (pure_early_return_bind m f) (at level 50, left associativity).
+Notation "m >>$ n" := (m >>$= fun _ => n) (at level 50, left associativity).
+
+Definition pure_early_return {A} (v : A + A) : A :=
+  match v with
+  | inl v' => v'
+  | inr v' => v'
+  end.
+
 (* Lift to monad with early return by wrapping exceptions *)
 (*val liftR : forall rv a r e. monad rv a e -> monadR rv a r e*)
 Definition liftR {rv A R E} (m : monad rv A E) : monadR rv A R E :=
@@ -178,19 +293,12 @@ Definition try_catchR {rv A R E1 E2} (m : monadR rv A R E1) (h : E1 -> monadR rv
       | inr e => h e
      end).
 
-(*val maybe_fail : forall 'rv 'a 'e. string -> maybe 'a -> monad 'rv 'a 'e*)
-Definition maybe_fail {rv A E} msg (x : option A) : monad rv A E :=
-match x with
-  | Some a => returnm a
-  | None => Fail msg
-end.
-
 (*val read_memt_bytes : forall 'rv 'a 'b 'e. Bitvector 'a, Bitvector 'b => read_kind -> 'a -> integer -> monad 'rv (list memory_byte * bitU) 'e*)
 Definition read_memt_bytes {rv A E} rk (addr : mword A) sz : monad rv (list memory_byte * bitU) E :=
-  Read_memt rk (Word.wordToNat (get_word addr)) (Z.to_nat sz) returnm.
+  Read_memt rk (mword_to_N addr) (Z.to_nat sz) returnm.
 
 (*val read_memt : forall 'rv 'a 'b 'e. Bitvector 'a, Bitvector 'b => read_kind -> 'a -> integer -> monad 'rv ('b * bitU) 'e*)
-Definition read_memt {rv A B E} `{ArithFact (B >=? 0)} rk (addr : mword A) sz : monad rv (mword B * bitU) E :=
+Definition read_memt {rv A E} rk (addr : mword A) sz : monad rv (mword (8 * sz) * bitU) E :=
   bind
     (read_memt_bytes rk addr sz)
     (fun '(bytes, tag) =>
@@ -201,10 +309,10 @@ Definition read_memt {rv A B E} `{ArithFact (B >=? 0)} rk (addr : mword A) sz : 
 
 (*val read_mem_bytes : forall 'rv 'a 'b 'e. Bitvector 'a, Bitvector 'b => read_kind -> 'a -> integer -> monad 'rv (list memory_byte) 'e*)
 Definition read_mem_bytes {rv A E} rk (addr : mword A) sz : monad rv (list memory_byte) E :=
-  Read_mem rk (Word.wordToNat (get_word addr)) (Z.to_nat sz) returnm.
+  Read_mem rk (mword_to_N addr) (Z.to_nat sz) returnm.
 
 (*val read_mem : forall 'rv 'a 'b 'e. Bitvector 'a, Bitvector 'b => read_kind -> 'a -> integer -> monad 'rv 'b 'e*)
-Definition read_mem {rv A B E} `{ArithFact (B >=? 0)} rk (addrsz : Z) (addr : mword A) sz : monad rv (mword B) E :=
+Definition read_mem {rv A E} rk (addrsz : Z) (addr : mword A) sz : monad rv (mword (8 * sz)) E :=
   bind
     (read_mem_bytes rk addr sz)
     (fun bytes =>
@@ -216,12 +324,12 @@ Definition excl_result {rv e} (_:unit) : monad rv bool e :=
   Excl_res k.
 
 Definition write_mem_ea {rv a E} wk (addrsz : Z) (addr: mword a) sz : monad rv unit E :=
- Write_ea wk (Word.wordToNat (get_word addr)) (Z.to_nat sz) (Done tt).
+ Write_ea wk (mword_to_N addr) (Z.to_nat sz) (Done tt).
 
 (*val write_mem : forall 'rv 'a 'b 'e. Bitvector 'a, Bitvector 'b =>
   write_kind -> integer -> 'a -> integer -> 'b -> monad 'rv bool 'e*)
-Definition write_mem {rv a b E} wk (addrsz : Z) (addr : mword a) sz (v : mword b) : monad rv bool E :=
-  match (mem_bytes_of_bits v, Word.wordToNat (get_word addr)) with
+Definition write_mem {rv a E} wk (addrsz : Z) (addr : mword a) sz (v : mword (8 * sz)) : monad rv bool E :=
+  match (mem_bytes_of_bits v, mword_to_N addr) with
     | (Some v, addr) =>
        Write_mem wk addr (Z.to_nat sz) v returnm
     | _ => Fail "write_mem"
@@ -229,12 +337,21 @@ Definition write_mem {rv a b E} wk (addrsz : Z) (addr : mword a) sz (v : mword b
 
 (*val write_memt : forall 'rv 'a 'b 'e. Bitvector 'a, Bitvector 'b =>
   write_kind -> 'a -> integer -> 'b -> bitU -> monad 'rv bool 'e*)
-Definition write_memt {rv a b E} wk (addr : mword a) sz (v : mword b) tag : monad rv bool E :=
-  match (mem_bytes_of_bits v, Word.wordToNat (get_word addr)) with
+Definition write_memt {rv a E} wk (addr : mword a) sz (v : mword (8 * sz)) tag : monad rv bool E :=
+  match (mem_bytes_of_bits v, mword_to_N addr) with
     | (Some v, addr) =>
        Write_memt wk addr (Z.to_nat sz) v tag returnm
     | _ => Fail "write_mem"
   end.
+
+Definition write_tag {rv a E} wk (addr : mword a) tag : monad rv bool E :=
+  let addr := mword_to_N addr in
+       Write_tag wk addr tag returnm.
+
+(* This alternate version is used in a few places, but should probably disappear *)
+Definition write_tag_bool {rv a E} (addr : mword a) tag : monad rv bool E :=
+  let addr := mword_to_N addr in
+       Write_tag Write_plain addr (bitU_of_bool tag) returnm.
 
 Definition read_reg {s rv a e} (reg : register_ref s rv a) : monad rv a e :=
   let k v :=
@@ -301,25 +418,29 @@ Local Open Scope bool_scope.
 Definition emitEvent {Regval A E} `{forall (x y : Regval), Decidable (x = y)} (m : monad Regval A E) (e : event Regval) : option (monad Regval A E) :=
  match (e, m) with
   | (E_read_mem rk a sz v, Read_mem rk' a' sz' k) =>
-     if read_kind_beq rk' rk && Nat.eqb a' a && Nat.eqb sz' sz then Some (k v) else None
+     if read_kind_beq rk' rk && N.eqb a' a && Nat.eqb sz' sz then Some (k v) else None
   | (E_read_memt rk a sz vt, Read_memt rk' a' sz' k) =>
-     if read_kind_beq rk' rk && Nat.eqb a' a && Nat.eqb sz' sz then Some (k vt) else None
+     if read_kind_beq rk' rk && N.eqb a' a && Nat.eqb sz' sz then Some (k vt) else None
   | (E_write_mem wk a sz v r, Write_mem wk' a' sz' v' k) =>
-     if write_kind_beq wk' wk && Nat.eqb a' a && Nat.eqb sz' sz && generic_eq v' v then Some (k r) else None
+     if write_kind_beq wk' wk && N.eqb a' a && Nat.eqb sz' sz && generic_eq v' v then Some (k r) else None
   | (E_write_memt wk a sz v tag r, Write_memt wk' a' sz' v' tag' k) =>
-     if write_kind_beq wk' wk && Nat.eqb a' a && Nat.eqb sz' sz && generic_eq v' v && generic_eq tag' tag then Some (k r) else None
+     if write_kind_beq wk' wk && N.eqb a' a && Nat.eqb sz' sz && generic_eq v' v && generic_eq tag' tag then Some (k r) else None
   | (E_read_reg r v, Read_reg r' k) =>
      if generic_eq r' r then Some (k v) else None
   | (E_write_reg r v, Write_reg r' v' k) =>
      if generic_eq r' r && generic_eq v' v then Some k else None
   | (E_write_ea wk a sz, Write_ea wk' a' sz' k) =>
-     if write_kind_beq wk' wk && Nat.eqb a' a && Nat.eqb sz' sz then Some k else None
+     if write_kind_beq wk' wk && N.eqb a' a && Nat.eqb sz' sz then Some k else None
   | (E_barrier bk, Barrier bk' k) =>
      if barrier_kind_beq bk' bk then Some k else None
   | (E_print m, Print m' k) =>
      if generic_eq m' m then Some k else None
   | (E_excl_res v, Excl_res k) => Some (k v)
-  | (E_choose descr v, Choose descr' k) => if generic_eq descr' descr then Some (k v) else None
+  | (E_choose descr ty v, Choose descr' ty' k) =>
+     match ChooseType_eq_dec ty' ty with
+     | left EQ => if generic_eq descr' descr then Some (k (eq_rect_r choose_type v EQ)) else None
+     | right _ => None
+     end
   | (E_footprint, Footprint k) => Some k
   | _ => None
 end.
